pulse/lib/pulse/lib/Pulse.Lib.SpinLock.fsti
@@ -16,6 +16,7 @@
 module Pulse.Lib.SpinLock
 
 open Pulse.Lib.Pervasives
+open Pulse.Lib.Stick
 
 module T = FStar.Tactics.V2
 
@@ -63,3 +64,27 @@ val lock_alive_inj (l:lock) (#p1 #p2 : perm) (#v1 #v2 : vprop)
   : stt_ghost unit emp_inames
               (lock_alive l #p1 v1 ** lock_alive l #p2 v2)
               (fun _ -> lock_alive l #p1 v1 ** lock_alive l #p2 v1)
+
+val iref_of (l:lock) : iref
+val iref_v_of (l:lock) (v:vprop) : vprop
+val lock_active (#[T.exact (`1.0R)] p:perm) (l:lock) : v:vprop { is_small v }
+
+val share_lock_active (#p:perm) (l:lock)
+  : stt_ghost unit emp_inames
+      (requires lock_active #p l)
+      (ensures fun _ -> lock_active #(p /. 2.0R) l ** lock_active #(p /. 2.0R) l)
+
+val gather_lock_active (#p1 #p2:perm) (l:lock)
+  : stt_ghost unit emp_inames
+      (requires lock_active #p1 l ** lock_active #p2 l)
+      (ensures fun _ -> lock_active #(p1 +. p2) l)
+
+val elim_inv_and_active_into_alive (l:lock) (v:vprop) (#p:perm)
+  : stt_ghost unit emp_inames
+      (requires emp)
+      (ensures fun _ -> (inv (iref_of l) (iref_v_of l v) ** lock_active #p l) @==> lock_alive l #p v)
+
+val elim_alive_into_inv_and_active (l:lock) (v:vprop) (#p:perm)
+  : stt_ghost unit emp_inames
+      (requires emp)
+      (ensures fun _ -> lock_alive l #p v @==> (inv (iref_of l) (iref_v_of l v) ** lock_active #p l))
