pulse/lib/pulse/lib/Pulse.Lib.SpinLockToken.fst
@@ -1,0 +1,81 @@
+(*
+   Copyright 2023 Microsoft Research
+
+   Licensed under the Apache License, Version 2.0 (the "License");
+   you may not use this file except in compliance with the License.
+   You may obtain a copy of the License at
+
+
+   Unless required by applicable law or agreed to in writing, software
+   distributed under the License is distributed on an "AS IS" BASIS,
+   WITHOUT WARRANTIES OR CONDITIONS OF ANY KIND, either express or implied.
+   See the License for the specific language governing permissions and
+   limitations under the License.
+*)
+
+module Pulse.Lib.SpinLockToken
+
+open Pulse.Lib.Pervasives
+open Pulse.Lib.Stick
+
+module T = Pulse.Lib.InvToken
+module L = Pulse.Lib.SpinLock
+
+noeq
+type lock (v:vprop) : Type u#4 = {
+  l : L.lock;
+
+  i : iref;
+
+  t1 : T.token (L.iref_of l) (L.iref_v_of l v);
+  t2 : T.token i (exists* (p:perm). L.lock_active #p l)
+}
+
+```pulse
+fn new_lock (v:vprop { is_big v })
+  requires v
+  returns _:lock v
+  ensures emp
+{
+  let l = L.new_lock v;
+  L.elim_alive_into_inv_and_active l v #1.0R;
+  elim_stick _ _;
+  let t1 = T.witness (L.iref_of l);
+  let i = new_invariant (exists* (p:perm). L.lock_active #p l);
+  let t2 = T.witness i;
+  let l = {
+    l;
+    i;
+    t1;
+    t2
+  };
+  l
+}
+```
+
+let lock_acquired (#v:vprop) (l:lock v) : vprop =
+  L.lock_acquired l.l
+
+```pulse
+fn acquire (#v:vprop) (l:lock v)
+  requires emp
+  ensures v ** lock_acquired l
+{
+  T.recall l.t2;
+  with_invariants l.i
+    returns _:unit
+    ensures inv l.i (exists* (p:perm). L.lock_active #p l.l) **
+            (exists* (p:perm). L.lock_active #p l.l) {
+    L.share_lock_active l.l
+  };
+
+  T.recall l.t1;
+  with p. assert (L.lock_active #p l.l);
+  L.elim_inv_and_active_into_alive l.l v #p;
+  elim_stick _ _;
+  drop_ (inv _ _);
+  L.acquire l.l;
+  fold (lock_acquired l);
+  drop_ (L.lock_alive l.l #p v)
+}
+```
